<section xml:id="Double-Angle_and_Half-Angle_Formulas">
  <title>Double-Angle and Half-Angle Formulas</title>
  <introduction>
    <p>
      In <xref ref="Right_Triangle_Trigonometry">Section</xref>
      we learned about <em>deviation</em>
      and how to calculate how far a wa&#699;a has traveled off course.
      For example,
      if a wa&#699;a traveled for one day of sailing at 5 knots or 120 nautical miles and was off course by 2 Houses or <m>22.5^{\circ}</m>,
      how far have they deviated?
    </p>
    <image>
<latex-image>
<![CDATA[\begin{tikzpicture}\node[above,yshift=0.15cm] at (0,0) {start};
\node[above right] at (22.5:1.2) {end};
\draw[line width=2pt,-stealth] (0,0) -- (22.5:1.2cm) node[midway,sloped,above] {120 miles};
\draw[dashed] (0,0) -- (1.10865543901,0);
\draw[dashed] (1.10865543901,0) -- (1.10865543901,0.459220118838)
node[midway,right,xshift=0.1cm] {\(y\)};
\draw ([shift=(0:0.2cm)]0,0) arc (0:22.5:0.2cm) node[midway,right,xshift=0.5cm,yshift=0.07cm] {\(22.5^{\circ}\)};
\draw ([shift=(22.5:-0.1cm)]0,0) pic {waa-top={waacolor}{-67.5}{0.1}};
\draw (1.04865543901,0) -- (1.04865543901,0.06) -- (1.10865543901,0.06);\end{tikzpicture}]]>
</latex-image>
    </image>
    <p>
      Using the methods of <xref ref="Right_Triangle_Trigonometry">Section</xref>,
      we concluded that the deviation was <m>y=120\cdot\sin22.5^{\circ}</m>.
      We then proceeded to obtain a numerical approximation because we could not obtain an exact value for <m>\sin22.5^{\circ}</m>.
      We are familiar with the value of trigonometric functions at
      <m>30, 45, 60^{\circ}</m> but not <m>22.5^{\circ}</m>.
      In this section,
      we will examine double and half angles and will be able to calculate the exact value of
      <m>\sin22.5^{\circ}</m> since <m>22.5=\frac{1}{2}\cdot45</m>.
    </p>
  </introduction>
  <subsection>
    <title>Double-Angle Formulas</title>
    <p>
      Recall the sum formula for sine:
      <men xml:id="eq_double-angle1">
        \sin (\alpha+\beta)=\sin \alpha \cos \beta + \cos \alpha \sin \beta
      </men>
    </p>
    <p>
      Consider the case when the two angles are equal.
      We will call this angle <m>\theta</m>,
      so let <m>\alpha=\theta</m> and <m>\beta=\theta</m>.
      Then <xref ref="eq_double-angle1">Eq</xref> becomes
      <md>
        <mrow>\sin(\theta+\theta)\amp =\amp \sin \theta \cos \theta + \cos \theta \sin \theta</mrow>
        <mrow>\sin (2\theta)\amp =\amp 2\sin \theta \cos \theta</mrow>
      </md>
    </p>
    <p>
      Thus we obtain a formula for sine of twice the angle <m>\theta</m>.
    </p>
    <p>
      \begin{mybox}[Double-Angle Formulas]
          <idx><h>double-angle formulas</h></idx>
      <md>
        <mrow>\sin 2\theta \amp =\amp  2\sin \theta \cos \theta</mrow>
      </md>
      <md>
        <mrow>\cos 2\theta \amp  =\amp   \cos^2 \theta - \sin^2 \theta</mrow>
        <mrow>\amp =\amp 1-2\sin^2 \theta</mrow>
        <mrow>\amp =\amp 2\cos^2 \theta-1</mrow>
      </md>
      <md>
        <mrow>\tan 2 \theta \amp =\amp  \frac{2\tan \theta}{1-\tan^2 \theta}</mrow>
      </md>
    </p>
    <p>
      \end{mybox} The proofs for the double-angle formulas for cosine and tangent are left as exercises.
    </p>
    <example>
      <statement>
        <p>
          If <m>\cos\theta=-\frac{4}{5}</m> and <m>\frac{\pi}{2}\lt \theta\lt \pi</m>,
          calculate <m>\sin2\theta</m>,
          <m>\cos2\theta</m>, and <m>\tan2\theta</m>.
        </p>
      </statement>
      <solution>
        <p>
          To compute <m>\cos2\theta</m>,
          notice there are three different formulas:
          <m>\cos2\theta=\cos^\theta-\sin^2\theta</m>,
          <m>\cos2\theta=1-2\sin^2\theta</m>,
          or <m>\cos2\theta=2\cos^2\theta-1</m>.
          Using any of the three equations will give us the correct answer,
          however, if we look at the information we are given,
          we know that <m>\cos\theta=-\frac{4}{5}</m> so it may be easier to use
          <m>\cos2\theta=2\cos^2\theta-1</m> since the first two equations require us to know <m>\sin\theta</m>.
          Thus
          <me>
            \cos2\theta=2\cos^2\theta-1=2\left(-\frac{4}{5}\right)^2-1=2\left(\frac{16}{25}\right)-1=\frac{32}{25}-\frac{25}{25}=\frac{7}{25}
          </me>
        </p>
        <p>
          To compute <m>\sin2\theta</m>,
          <m>\tan2\theta</m>,
          or using the other equations for <m>\cos2\theta</m>,
          we will need to compute <m>\sin\theta</m> and <m>\tan\theta</m>.
          To do this, we will draw the triangle formed from
          <m>\cos\theta=-\frac{4}{5}</m> where <m>-\frac{\pi}{2}\lt \theta\lt \pi</m>.
        </p>
        <image>
<latex-image>
<![CDATA[\begin{tikzpicture}\draw[<->] (-4.5,0)--(0.5,0) node[right]{\(x\)};
\draw[<->] (0,-0.5)--(0,3.5) node[above]{\(y\)};
\draw[line width=1pt] (0,0) -- (-4,0) node[midway,below]{-4};
\draw[line width=1pt] (-4,0) -- (-4,3) node[midway,left]{y};
\draw[line width=1pt] (-4,3) -- (0,0) node[midway,above]{5};
\draw (143.130102354:1) arc (143.130102354:180:1) node[midway, left,xshift=-1,yshift=4] {\(\theta\)};
\draw (-3.6,0) -- (-3.6,0.4) -- (-4,0.4);\end{tikzpicture}]]>
</latex-image>
        </image>
        <p>
          Using the Pythagorean Theorem,
          we can solve the triangle:
          <md>
            <mrow>(-4)^2+y^2\amp =\amp 5^2</mrow>
            <mrow>16+y^2\amp =\amp 25</mrow>
            <mrow>y^2\amp =\amp 9</mrow>
            <mrow>y\amp =\amp 3</mrow>
          </md>
        </p>
        <p>
          Using the right triangle, we can now find an expression for
          <me>
            \sin\theta=\frac{\mbox{opposite} }{\mbox{hypotenuse} }=\frac{3}{5}
          </me>
          and
          <me>
            \tan\theta=\frac{\mbox{opposite} }{\mbox{adjacent} }=\frac{3}{-4}=-\frac{3}{4}
          </me>
        </p>
        <p>
          Using the Double-Angle Formula, we get
          <me>
            \sin2\theta=2\sin\theta\cos\theta=2\left(\frac{3}{5}\right)\left(-\frac{4}{5}\right)=-\frac{24}{25}
          </me>
          and
          <me>
            \tan2\theta=\frac{2\tan\theta}{1-\tan^2\theta}=\frac{2\left(-\frac{3}{4}\right)}{1-\left(-\frac{3}{4}\right)^2}=\frac{-\frac{6}{4}}{1-\frac{9}{16}}=\frac{-\frac{6}{4}}{\frac{16}{16}-\frac{9}{16}}=\frac{-\frac{6}{4}}{\frac{7}{16}}=-\frac{6}{4}\cdot\frac{16}{7}=-\frac{24}{7}
          </me>
        </p>
      </solution>
    </example>
    <example>
      <statement>
        <p>
          Write <m>\cos(3\theta)</m> in terms of <m>\sin\theta</m>.
        </p>
      </statement>
      <solution>
        <md>
          <mrow>\sin(3\theta)\amp =\sin(2\theta+\theta)</mrow>
          <mrow>\amp =\sin(2\theta)\cos\theta+\cos(2\theta)\sin\theta\amp \amp \mbox{sum formula}</mrow>
          <mrow>\amp =(2\sin\theta\cos\theta)\cos\theta+(\cos^2\theta-\sin^2\theta)\sin\theta\amp \amp \mbox{double-angle formula}</mrow>
          <mrow>\amp =2\sin\theta\cos^2\theta+\sin\theta\cos^2\theta-\sin^3\theta</mrow>
          <mrow>\amp =3\sin\theta\cos^2\theta-\sin^3\theta</mrow>
          <mrow>\amp =3\sin\theta(1-\sin^2\theta)-\sin^3\theta\amp \amp \mbox{Pythagorean Identity}</mrow>
          <mrow>\amp =3\sin\theta-3\sin^3\theta-\sin^3\theta</mrow>
          <mrow>\amp =3\sin\theta-4\sin^3\theta</mrow>
        </md>
      </solution>
    </example>
  </subsection>
  <subsection>
    <title>Reducing Powers Formulas</title>
    <p>
      You may notice that the double angle formula for cosine takes a trigonometric function and expresses it in terms of the square of a trigonometric function.
      If we rearrange the terms,
      we can obtain formula for reducing the powers of sine, cosine,
      and tangent expressions with even powers in terms of only cosine.
      These formulas come in handy in calculus.
    </p>
    <p>
      \begin{mybox}[Formulas for Reducing Powers]<idx><h>reducing powers formulas</h></idx>
      <me>
        \sin^2\theta=\frac{1-\cos(2\theta)}{2}
      </me>
      <me>
        \cos^2\theta=\frac{1+\cos(2\theta)}{2}
      </me>
      <me>
        \tan^2\theta=\frac{1-\cos(2\theta)}{1+\cos(2\theta)}
      </me>
    </p>
    <p>
      \end{mybox}
    </p>
    <proof>
      <p>
        To prove the first formula,
        solve for <m>\sin^2\theta</m> in the Double-Angle Formula <m>\cos2\theta=1-2\sin^2\theta</m>.
        The second formula is obtained similarly by solving for
        <m>\cos^2\theta</m> in the formula <m>\cos2\theta=2\cos^2\theta-1</m>.
        The first two formula can be used to obtain the third formula
        <me>
          \tan^2\theta=\frac{\sin^2\theta}{\cos^2\theta}=\frac{\dfrac{1-\cos(2\theta)}{2}}{\dfrac{1+\cos(2\theta)}{2}}=\frac{1-\cos(2\theta)}{1+\cos(2\theta)}
        </me>
      </p>
    </proof>
    <example>
      <statement>
        <p>
          Write <m>\sin^4\theta</m> as an expression that does not involve powers of sine or cosine greater than 1.
        </p>
      </statement>
      <solution>
        <p>
          We will use the power reduction formula twice.
          <md>
            <mrow>\sin^2\theta \amp = (\sin^2\theta)^2</mrow>
            <mrow>\amp =\left(\frac{1-\cos(2\theta)}{2}\right)^2\amp \amp \mbox{reducing powers}</mrow>
            <mrow>\amp =\frac{1}{4}\left(1-2\cos(2\theta)+\cos^2(2\theta)\right)</mrow>
            <mrow>\amp =\frac{1}{4}\left(1-2\cos(2\theta)+\frac{1+\cos(4\theta)}{2}\right)\amp \amp \mbox{reducing powers}</mrow>
            <mrow>\amp =\frac{1}{4}\left(1-2\cos(2\theta)+\frac{1}{2}+\frac{\cos(4\theta)}{2}\right)</mrow>
            <mrow>\amp =\frac{1}{4}\left(\frac{3}{2}-2\cos(2\theta)+\frac{\cos(4\theta)}{2}\right)</mrow>
            <mrow>\amp =\frac{3}{8}-\frac{1}{2}\cos(2\theta)+\frac{\cos(4\theta)}{8}</mrow>
          </md>
        </p>
      </solution>
    </example>
  </subsection>
  <subsection>
    <title>Half-Angle Formulas</title>
    <p>
      Another set of useful formulas are the half-angle formulas. \begin{mybox}[Half-Angle Formulas]<idx><h>Half-Angle Formulas</h><h>for Sine</h></idx>
          <idx><h>Half-Angle Formulas</h><h>for Cosine</h></idx>
          <idx><h>Half-Angle Formulas</h><h>for Tangent</h></idx>
      <md>
        <mrow>\sin\frac{\theta}{2}\amp =\pm\sqrt{\frac{1-\cos\theta}{2}},\amp \cos\frac{\theta}{2}\amp =\pm\sqrt{\frac{1+\cos\theta}{2}},\amp \tan\frac{\theta}{2}\amp =\pm\sqrt{\frac{1-\cos\theta}{1+\cos\theta}}</mrow>
      </md>
    </p>
    <p>
      The choice of the + or - sign depends on the Quadrant in which <m>\theta/2</m> lies. \end{mybox}
    </p>
    <proof>
      <p>
        We take the square root on both sides of the Formulas for Reducing Powers and halve the angle (<m>\theta</m> becomes
        <m>\frac{\theta}{2}</m> and <m>2\theta</m> becomes <m>\theta</m>) to arrive at our formulas.
      </p>
    </proof>
    <example>
      <title>Deviation</title>
      <statement>
        <p>
          We are now ready to revisit the problem posed at the start of this section when we were give that a wa&#699;a traveling 120 NM deviates by
          <m>22.5^{\circ}</m> and we asked to determine the exact value of how far it deviated.
          Houses or <m>22.5^{\circ}</m>,
          how far have they deviated?
        </p>
        <image>
<latex-image>
<![CDATA[\begin{tikzpicture}\node[above,yshift=0.15cm] at (0,0) {start};
\node[above right] at (22.5:1.2) {end};
\draw[line width=2pt,-stealth] (0,0) -- (22.5:1.2cm) node[midway,sloped,above] {120 miles};
\draw[dashed] (0,0) -- (1.10865543901,0);
\draw[dashed] (1.10865543901,0) -- (1.10865543901,0.459220118838)
node[midway,right,xshift=0.1cm] {\(y\)};
\draw ([shift=(0:0.2cm)]0,0) arc (0:22.5:0.2cm) node[midway,right,xshift=0.5cm,yshift=0.07cm] {\(22.5^{\circ}\)};
\draw ([shift=(22.5:-0.1cm)]0,0) pic {waa-top={waacolor}{(-67.5)}{0.1}};
\draw (1.04865543901,0) -- (1.04865543901,0.06) -- (1.10865543901,0.06);\end{tikzpicture}]]>
</latex-image>
        </image>
      </statement>
      <solution>
        <p>
          We know the deviation is
          <me>
            y=120\cdot\sin22.5^{\circ}=120\cdot\sin\left(\frac{45}{2}\right)^{\circ}=120\cdot\sqrt{\frac{1-\cos45^{\circ}}{2}}=120\cdot\sqrt{\frac{1-\frac{\sqrt{2}}{2}}{2}}
          </me>
          <me>
            =120\cdot\sqrt{\frac{\frac{2}{2}-\frac{\sqrt{2}}{2}}{2}}=120\cdot\sqrt{\frac{2-\sqrt{2}}{4}}=\frac{120}{2}\cdot\sqrt{2-\sqrt{2}}=60\cdot\sqrt{2-\sqrt{2}}
          </me>
        </p>
        <p>
          Thus we have found the exact value of <m>120\cdot\sin22.5^{\circ}=60\cdot\sqrt{2-\sqrt{2}}\mbox{ NM}</m>.
        </p>
      </solution>
    </example>
    <example xml:id="ex_half-angle">
      <statement>
        <p>
          Given <m>\sin\theta=-\frac{5}{13}</m> and <m>\theta</m> lies in Quadrant III, find the exact value of
          <ol>
            <li>
              <p>
                <m>\sin\frac{\theta}{2}</m>
              </p>
            </li>
            <li>
              <p>
                <m>\cos\frac{\theta}{2}</m>
              </p>
            </li>
            <li>
              <p>
                <m>\tan\frac{\theta}{2}</m>
              </p>
            </li>
          </ol>
        </p>
      </statement>
      <solution>
        <p>
          Notice the Half-Angle Formulas all require us to know
          <m>\cos\theta</m> so we begin by drawing the triangle formed from
          <m>\sin\theta=-\frac{5}{13}</m> and <m>\theta</m> in Quadrant III.
        </p>
        <image>
<latex-image>
<![CDATA[\begin{tikzpicture}\draw[<->] (-13,0)--(1,0) node[right]{\(x\)};
\draw[<->] (0,-6)--(0,1) node[above]{\(y\)};
\draw[line width=1pt] (0,0) -- (-12,0) node[midway,above]{-x};
\draw[line width=1pt] (-12,0) -- (-12,-5) node[midway,left]{-5};
\draw[line width=1pt] (-12,-5) -- (0,0) node[midway,below]{13};
\draw (180:2) arc (180:202.619864948:2) node[midway, left,xshift=-4,yshift=-3] {\(\theta\)};
\draw (-11,0) -- (-11,-1) -- (-12,-1);\end{tikzpicture}]]>
</latex-image>
        </image>
        <p>
          Using the Pythagorean Theorem,
          we can solve the triangle:
          <md>
            <mrow>x^2+(-5)^2\amp =\amp 13^2</mrow>
            <mrow>x^2+25\amp =\amp 169</mrow>
            <mrow>x^2\amp =\amp 144</mrow>
            <mrow>x\amp =\amp 12</mrow>
          </md>
        </p>
        <p>
          Thus we have
          <me>
            \cos\theta=-\frac{12}{13}
          </me>
        </p>
        <p>
          Next, since <m>\theta</m> is in Quadrant III, <m>180^{\circ}\lt \theta\lt 270^{\circ}</m>,
          so dividing by 2 gives us <m>\frac{180^{\circ}}{2}\lt \frac{\theta}{2}\lt \frac{270^{\circ}}{2}</m> or <m>90^{\circ}\lt \frac{\theta}{2}\lt 135^{\circ}</m>.
          Therefore, we conclude that <m>\frac{\theta}{2}</m> lies in Quadrant II.
          <ol>
            <li>
              <p>
                To calculate <m>\sin\frac{\theta}{2}</m>,
                we first note that because <m>\frac{\theta}{2}</m> lies in Quadrant II,
                <m>\sin\frac{\theta}{2}>0</m> so we will choose the positive (+) sign in the Half-Angle Formula:
                <md>
                  <mrow>\sin\frac{\theta}{2}\amp =\amp \sqrt{\frac{1-\cos\theta}{2}}</mrow>
                  <mrow>\amp =\amp \sqrt{\frac{1-\left(-\frac{12}{13}\right)}{2}}</mrow>
                  <mrow>\amp =\amp \sqrt{\frac{1+\frac{12}{13}}{2}}</mrow>
                  <mrow>\amp =\amp \sqrt{\frac{\frac{13}{13}+\frac{12}{13}}{2}}</mrow>
                  <mrow>\amp =\amp \sqrt{\frac{\frac{25}{13}}{2}}</mrow>
                  <mrow>\amp =\amp \sqrt{\frac{25}{26}}</mrow>
                </md>
              </p>
            </li>
            <li>
              <p>
                Since <m>\frac{\theta}{2}</m> is in Quadrant II, we know that
                <m>\cos\frac{\theta}{2}\lt 0</m> so we will choose the negative (-) sign in the Half-Angle Formula:
                <md>
                  <mrow>\cos\frac{\theta}{2}\amp =\amp -\sqrt{\frac{1+\cos\theta}{2}}</mrow>
                  <mrow>\amp =\amp -\sqrt{\frac{1+\left(-\frac{12}{13}\right)}{2}}</mrow>
                  <mrow>\amp =\amp -\sqrt{\frac{1-\frac{12}{13}}{2}}</mrow>
                  <mrow>\amp =\amp -\sqrt{\frac{\frac{13}{13}-\frac{12}{13}}{2}}</mrow>
                  <mrow>\amp =\amp -\sqrt{\frac{\frac{1}{13}}{2}}</mrow>
                  <mrow>\amp =\amp -\sqrt{\frac{1}{26}}</mrow>
                </md>
              </p>
            </li>
            <li>
              <p>
                Since <m>\frac{\theta}{2}</m> is in Quadrant II, we know that
                <m>\tan\frac{\theta}{2}\lt 0</m> so we will choose the negative (-) sign in the Half-Angle Formula:
                <md>
                  <mrow>\tan\frac{\theta}{2}\amp =\amp -\sqrt{\frac{1-\cos\theta}{1+\cos\theta}}</mrow>
                  <mrow>\amp =\amp -\sqrt{\frac{1-\left(-\frac{12}{13}\right)}{1+\left(-\frac{12}{13}\right)}}</mrow>
                  <mrow>\amp =\amp -\sqrt{\frac{1+\frac{12}{13}}{1-\frac{12}{13}}}</mrow>
                  <mrow>\amp =\amp -\sqrt{\frac{\frac{13}{13}+\frac{12}{13}}{\frac{13}{13}-\frac{12}{13}}}</mrow>
                  <mrow>\amp =\amp -\sqrt{\frac{\frac{25}{13}}{\frac{1}{13}}}</mrow>
                  <mrow>\amp =\amp -\sqrt{\frac{25}{13}\cdot\frac{13}{1}}</mrow>
                  <mrow>\amp =\amp -\sqrt{25}</mrow>
                  <mrow>\amp =\amp -5</mrow>
                </md>
              </p>
            </li>
          </ol>
        </p>
      </solution>
    </example>
    <p>
      We can derive another formula for
      <m>\tan\frac{\theta}{2}</m> that does not involve <m>\pm</m>: \begin{mybox}[Half-Angle Formulas for Tangent]<idx><h>Half-Angle Formulas</h><h>for Tangent</h></idx>
      <me>
        \tan\frac{\theta}{2}=\pm\sqrt{\frac{1-\cos\theta}{1+\cos\theta}}=\frac{1-\cos\theta}{\sin\theta}=\frac{\sin\theta}{1+\cos\theta}
      </me>
    </p>
    <p>
      \end{mybox}
    </p>
    <proof>
      <p>
        We begin by first multiplying both sides of the Sine formula for Reducing Powers by 2 and halving the angle:
        <me>
          1-\cos\theta=2\sin^2\left(\frac{\theta}{2}\right)
        </me>
        and applying the double-angle formula to:
        <me>
          \sin\theta=\sin2\cdot\frac{\theta}{2}=2\sin\frac{\theta}{2}\cos\frac{\theta}{2}
        </me>
      </p>
      <p>
        Diving the two preceding results
        <me>
          \frac{1-\cos\theta}{\sin\theta}=\frac{2\sin^2\left(\frac{\theta}{2}\right)}{2\sin\frac{\theta}{2}\cos\frac{\theta}{2}}=\frac{\sin\frac{\theta}{2}}{\cos\frac{\theta}{2}}=\tan\frac{\theta}{2}
        </me>
      </p>
      <p>
        Thus
        <me>
          \tan\frac{\theta}{2}=\frac{1-\cos\theta}{\sin\theta}
        </me>
      </p>
      <p>
        Similarly, it can be shown that
        <me>
          \tan\frac{\theta}{2}=\frac{\sin\theta}{1+\cos\theta}
        </me>
      </p>
    </proof>
    <example>
      <statement>
        <p>
          Calculate <m>\tan\frac{\theta}{2}</m> from <xref ref="ex_half-angle">Example</xref> using the above formula.
        </p>
      </statement>
      <solution>
        <me>
          \tan\frac{\theta}{2}=\frac{1-\cos\theta}{\sin\theta}=\frac{1-\left(-\frac{12}{13}\right)}{-\frac{5}{13}}=\frac{\frac{25}{13}}{-\frac{5}{13}}=\frac{25}{13}\cdot\left(-\frac{13}{5}\right)=-5
        </me>
      </solution>
    </example>
    <p>
      Note: We obtained the same result for
      <m>\tan\frac{\theta}{2}</m> as we did in <xref ref="ex_half-angle">Example</xref>.
      In this example, we did not have to determine if
      <m>\tan\frac{\theta}{2}</m> was positive or negative, however,
      we do need to know the values of both
      <m>\sin\theta</m> and <m>\cos\theta</m>.
    </p>
    <exercise xml:id="ex-3_3">
      <statement>
        <me>
          \cos2\theta=\cos^2\theta-\sin^2\theta
        </me>
        
<task>
<introduction>
  <p>
    Use the Pythagorean identity (<m>\sin^2\theta+\cos^2\theta=1</m>) and the result from <xref ref="x3_3-ex1">Exercise</xref> to prove
          <me>
            \cos2\theta=1-2\sin^2\theta
          </me>
  </p>
</introduction>
<statement>
<p>
Use the Pythagorean identity (<m>\sin^2\theta+\cos^2\theta=1</m>) and the result from <xref ref="x3_3-ex1">Exercise</xref> to prove
          <me>
            \cos2\theta=1-2\sin^2\theta
          </me>
      </p>
    </statement>
    <answer>
      <p>
        MYANSWER
      </p>
    </answer>
  </task>
        
<task>
<introduction>
  <p>
    Use the Pythagorean identify (<m>\sin^2\theta+\cos^2\theta=1</m>) and the result from <xref ref="x3_3-ex1">Exercise</xref> to prove
          <me>
            \cos2\theta=2\cos^2\theta-1
          </me>
  </p>
</introduction>
<statement>
<p>
Use the Pythagorean identify (<m>\sin^2\theta+\cos^2\theta=1</m>) and the result from <xref ref="x3_3-ex1">Exercise</xref> to prove
          <me>
            \cos2\theta=2\cos^2\theta-1
          </me>
      </p>
    </statement>
    <answer>
      <p>
        MYANSWER
      </p>
    </answer>
  </task>
        
<task>
<introduction>
  <p>
    Use the sum formula,
          <m>\tan(\alpha+\beta)=\frac{\tan\alpha+\tan\beta}{1-\tan\alpha\tan\beta}</m>,
          to prove the double angle formula for tangent:
          <me>
            \tan2\theta=\frac{2\tan\theta}{1-\tan^2\theta}
          </me>
  </p>
</introduction>
<statement>
<p>
Use the sum formula,
          <m>\tan(\alpha+\beta)=\frac{\tan\alpha+\tan\beta}{1-\tan\alpha\tan\beta}</m>,
          to prove the double angle formula for tangent:
          <me>
            \tan2\theta=\frac{2\tan\theta}{1-\tan^2\theta}
          </me>
      </p>
    </statement>
    <answer>
      <p>
        MYANSWER
      </p>
    </answer>
  </task>
        
<introduction>
  <p>
    Find the exact value of i)
          <m>\sin2\theta</m>, ii) <m>\cos2\theta</m>,
          and iii) <m>\tan2\theta</m> if 
  </p>
</introduction>
  <task>
    <statement>
      <p>
        
          <m>\cos\theta=\frac{-3}{5}</m> and <m>\theta</m> is in Quadrant III
      </p>
    </statement>
    <answer>
      <p>
        MYANSWER
      </p>
    </answer>
  </task>
        <p>
          \task <m>\sin\theta=-\frac{8}{17}</m> and <m>270^{\circ}\lt \theta\lt 360^{\circ}</m>
        </p>
        <p>
          \end{tasks}
        </p>
        
<introduction>
  <p>
    Using the Half-Angle Formula,
          find the exact value of 
  </p>
</introduction>
  <task>
    <statement>
      <p>
         <m>\tan315^{\circ}</m>
      </p>
    </statement>
    <answer>
      <p>
        MYANSWER
      </p>
    </answer>
  </task>
        <p>
          \task <m>\sin150^{\circ}</m>
        </p>
        <p>
          \task <m>\tan225^{\circ}</m>
        </p>
        <p>
          \task <m>\cos30^{\circ}</m>
        </p>
        <p>
          \task <m>\cos\frac{\pi}{8}</m>
        </p>
        <p>
          \task <m>\tan\frac{11\pi}{12}</m>
        </p>
        <p>
          \task <m>\sin\frac{7\pi}{12}</m>
        </p>
        <p>
          \task <m>\cos\frac{3\pi}{8}</m>
        </p>
        <p>
          \end{tasks}
        </p>
        
<introduction>
  <p>
    Use the Half-Angle Formulas to find the exact values of i) <m>\sin\frac{\theta}{2}</m>,
          ii) <m>\cos\frac{\theta}{2}</m>,
          and iii) <m>\tan\frac{\theta}{2}</m> if 
  </p>
</introduction>
  <task>
    <statement>
      <p>
        
          <m>\tan\theta=-\frac{4}{3}</m> and <m>\theta</m> is in Quadrant II
      </p>
    </statement>
    <answer>
      <p>
        MYANSWER
      </p>
    </answer>
  </task>
        <p>
          \task <m>\cos\theta=\frac{2}{3}</m> and <m>\frac{3\pi}{4}\lt \theta\lt 2\pi</m> \end{tasks}
        </p>
      </statement>
    </exercise>
  </subsection>
</section>
