<?xml version="1.0" encoding="UTF-8"?>
<section xml:id="Product-to-Sum_and_Sum-to-Product_Formulas">
  <title>Product-to-Sum and Sum-to-Product Formulas</title>
  <p>
    *needs motivation/intro, needs examples,
    and needs to expand on the math*
  </p>
  <p>
    \begin{mybox}[Product-to-Sum Formulas]
        <idx><h>product-to-sum formulas</h></idx>
    <me>
      \sin\alpha\cos\beta=\frac{1}{2}[\sin(\alpha+\beta)+\sin(\alpha-\beta)]
    </me>
    <me>
      \cos\alpha\sin\beta=\frac{1}{2}[\sin(\alpha+\beta)-\sin(\alpha-\beta)]
    </me>
    <me>
      \cos\alpha\cos\beta=\frac{1}{2}[\cos(\alpha+\beta)+\cos(\alpha-\beta)]
    </me>
    <me>
      \sin\alpha\sin\beta=\frac{1}{2}[\cos(\alpha-\beta)-\cos(\alpha+\beta)]
    </me>
  </p>
  <p>
    \end{mybox}
  </p>
  <proof>
    <p>
      We add the sum and difference formula for cosine:
      <me>
        \begin{array}{rcl} \cos(\alpha+\beta)\amp =\amp \cos\alpha\cos\beta-\sin\alpha\sin\beta\\ +\cos(\alpha-\beta)\amp =\amp \cos\alpha\cos\beta+\sin\alpha\sin\beta\\ \hline \end{array}
      </me>
    </p>
    <p>
      Dividing both sides by 2, we get
      <me>
        \frac{1}{2}[\cos(\alpha+\beta)+\cos(\alpha-\beta)]=\cos\alpha\cos\beta
      </me>
    </p>
    <p>
      We add the sum and difference formula for sine:
      <me>
        \begin{array}{rcl} \sin(\alpha+\beta)\amp =\amp \sin\alpha\cos\beta+\cos\alpha\sin\beta\\ +\sin(\alpha-\beta)\amp =\amp \sin\alpha\cos\beta-\cos\alpha\sin\beta\\ \hline \end{array}
      </me>
    </p>
    <p>
      Dividing both sides by 2, we get
      <me>
        \frac{1}{2}[\sin(\alpha+\beta)+\sin(\alpha-\beta)=\sin\alpha\cos\beta
      </me>
    </p>
    <p>
      We subtract the sum and difference formula for sine:
      <me>
        \begin{array}{rcl} \sin(\alpha+\beta)\amp =\amp \sin\alpha\cos\beta+\cos\alpha\sin\beta\\ -\sin(\alpha-\beta)\amp =\amp \sin\alpha\cos\beta-\cos\alpha\sin\beta\\ \hline \end{array}
      </me>
    </p>
    <p>
      Dividing both sides by 2, we get
      <me>
        \frac{1}{2}[\sin(\alpha+\beta)-\sin(\alpha-\beta)=\sin\beta\cos\alpha
      </me>
    </p>
    <p>
      We subtract the difference and sum formula for cosine:
      <me>
        \begin{array}{rcl} \cos(\alpha-\beta)\amp =\amp \cos\alpha\cos\beta+\sin\alpha\sin\beta\\ -\cos(\alpha+\beta)\amp =\amp \cos\alpha\cos\beta-\sin\alpha\sin\beta\\ \hline \end{array}
      </me>
    </p>
    <p>
      Dividing both sides by 2, we get
      <me>
        \frac{1}{2}[\cos(\alpha-\beta)-\cos(\alpha+\beta)]=\sin\alpha\sin\beta
      </me>
    </p>
  </proof>
  <example>
    <statement>
      <p>
        Express the product of <m>\cos2x\cos5x</m> as a sum or difference of sine and cosine with no products **fix wording**
      </p>
    </statement>
    <solution>
      <p>
        Using the formula we get
        <md>
          <mrow>\cos2x\cos5x\amp =\amp \frac{1}{2}[\cos(2x+5x)+\cos(2x-5x)]</mrow>
          <mrow>\amp =\amp \frac{1}{2}[\cos(7x)+\cos(-3x)]</mrow>
        </md>
      </p>
      <p>
        Since cosine is even, <m>\cos(-3x)=\cos3x</m>.
        Thus,
        <me>
          \cos2x\cos5x=\frac{1}{2}[\cos(7x)+\cos(3x)]
        </me>
      </p>
    </solution>
  </example>
  <p>
    \begin{mybox}[Sum-to-Product Formula]
        <idx><h>sum-to-product formula</h></idx>
    <md>
      <mrow>\sin\alpha+\sin\beta\amp =\amp 2\sin\left(\frac{\alpha+\beta}{2}\right)\cos\left(\frac{\alpha-\beta}{2}\right)</mrow>
      <mrow>\sin\alpha-\sin\beta\amp =\amp 2\cos\left(\frac{\alpha+\beta}{2}\right)\sin\left(\frac{\alpha-\beta}{2}\right)</mrow>
      <mrow>\cos\alpha+\cos\beta\amp =\amp 2\cos\left(\frac{\alpha+\beta}{2}\right)\cos\left(\frac{\alpha-\beta}{2}\right)</mrow>
      <mrow>\cos\alpha-\cos\beta\amp =\amp -2\sin\left(\frac{\alpha+\beta}{2}\right)\sin\left(\frac{\alpha-\beta}{2}\right)</mrow>
    </md>
  </p>
  <p>
    \end{mybox}
  </p>
  <proof>
    <p>
      We first let <m>\alpha=\frac{u+v}{2}</m> and <m>\beta=\frac{u-v}{2}</m>.
      Then
      <me>
        \alpha+\beta=\frac{u+v}{2}+\frac{u-v}{2}=\frac{2u}{2}=u
      </me>
      and
      <me>
        \alpha-\beta=\frac{u+v}{2}-\frac{u-v}{2}=\frac{2v}{2}=v
      </me>
    </p>
    <p>
      Substituting these values for <m>\alpha</m>,
      <m>\beta</m>, <m>\alpha+\beta</m>,
      and <m>\alpha-\beta</m> into the Product-to-Sum Formulas, we get
      <md>
        <mrow>\sin\left(\frac{u+v}{2}\right)\cos\left(\frac{u-v}{2}\right)\amp =\amp \frac{1}{2}[\sin(u)+\sin(v)]</mrow>
        <mrow>\cos\left(\frac{u+v}{2}\right)\sin\left(\frac{u-v}{2}\right)\amp =\amp \frac{1}{2}[\sin(u)-\sin(v)]</mrow>
        <mrow>\cos\left(\frac{u+v}{2}\right)\cos\left(\frac{u-v}{2}\right)\amp =\amp \frac{1}{2}[\cos(u)+\cos(v)]</mrow>
        <mrow>\sin\left(\frac{u+v}{2}\right)\sin\left(\frac{u-v}{2}\right)\amp =\amp \frac{1}{2}[\cos(v)-\cos(u)]</mrow>
      </md>
    </p>
    <p>
      Multiplying both sides by 2 and replacing <m>u</m> with <m>\alpha</m> and <m>v</m> with <m>\beta</m> we end up with the Sum-to-Product Formula. (multiply the last equation by -1)
    </p>
    <p>
      ***reword***
    </p>
  </proof>
  <p>
    Example:
  </p>
  <p>
    GPS. "<url href="\1"/>
  </p>
</section>